several styles of parallel increment, with locks and invariants, etc. With some workarounds for checker issues

pulse/share/steel/examples/pulse/by-example/ParallelIncrement.fst
@@ -143,3 +143,355 @@ ensures pts_to x ('i + 2)
     GR.free right;
 }
 ```
+
+assume
+val atomic_increment (r:ref int) (#i:erased int)
+  : stt_atomic unit emp_inames 
+    (pts_to r i)
+    (fun _ -> pts_to r (i + 1))
+     
+module F = Pulse.Lib.FlippableInv
+
+```pulse
+fn atomic_increment_f2
+        (x: ref int)
+        (#pred #qpred: int -> vprop)
+        (l:inv (exists* v. pts_to x v ** pred v))
+        (f: (v:int -> vq:int -> stt_ghost unit emp_inames 
+                  (pred v ** qpred vq ** pts_to x (v + 1))
+                  (fun _ -> pred (v + 1) ** qpred (vq + 1) ** pts_to x (v + 1))))
+requires qpred 'i
+ensures qpred ('i + 1)
+{
+  with_invariants l {
+    with v. _;
+    atomic_increment x;
+    f v 'i;
+  }
+}
+```
+
+open Pulse.Lib.Stick.Util
+module FA = Pulse.Lib.Forall.Util
+module I = Pulse.Lib.Stick.Util
+```pulse
+fn atomic_increment_f3
+        (x: ref int)
+        (#pred #qpred: int -> vprop)
+        (l:inv (exists* v. pts_to x v ** pred v))
+requires
+  qpred 'i **
+  (forall* v vq.
+     (pred v ** qpred vq ** pts_to x (v + 1)) @==>
+     (pred (v + 1) ** qpred (vq + 1) ** pts_to x (v + 1)))
+ensures qpred ('i + 1)
+{
+  with_invariants l {
+    with v. _;
+    atomic_increment x;
+    FA.elim #_ #(fun v -> forall* vq. (pred v ** qpred vq ** pts_to x (v + 1)) @==>
+                                      (pred (v + 1) ** qpred (vq + 1) ** pts_to x (v + 1))) v;
+
+    FA.elim #_ #(fun vq -> (pred v ** qpred vq ** pts_to x (v + 1)) @==>
+                           (pred (v + 1) ** qpred (vq + 1) ** pts_to x (v + 1))) 'i;
+    I.elim _ _;
+  }
+}
+```
+#pop-options
+```pulse
+fn atomic_increment_f4
+        (x: ref int)
+        (#invp : vprop)
+        (#pred #qpred: int -> vprop)
+        (l:inv invp)
+        (f: (v:int -> vq:int -> stt_ghost unit emp_inames 
+                  (pred v ** qpred vq ** pts_to x (v + 1))
+                  (fun _ -> pred (v + 1) ** qpred (vq + 1) ** pts_to x (v + 1))))
+requires
+  qpred 'i **
+  (invp @==> (exists* v. pts_to x v ** pred v)) ** 
+  ((exists* v. pts_to x v ** pred v) @==> invp)
+ensures qpred ('i + 1)
+{
+  with_invariants l {
+    I.elim invp _;
+    atomic_increment x;
+    f _ 'i;
+    I.elim (exists* v. pts_to x v ** pred v) invp;
+  }
+}
+```
+
+assume
+val atomic_read (r:ref int) (#i:erased int)
+  : stt_atomic int emp_inames 
+    (pts_to r #(half_perm full_perm) i)
+    (fun v -> pts_to r #(half_perm full_perm) v ** pure (reveal i == v))
+
+let cond b (p q:vprop) = if b then p else q
+assume
+val elim_cond_true (b:bool) (p q:vprop)
+  : stt_ghost unit emp_inames 
+    (cond b p q ** pure (b == true))
+    (fun _ -> p)
+
+assume
+val elim_cond_false (b:bool) (p q:vprop)
+  : stt_ghost unit emp_inames 
+    (cond b p q ** pure (b == false))
+    (fun _ -> q)
+
+assume
+val intro_cond_false (p q:vprop)
+  : stt_ghost unit emp_inames 
+    q (fun _ -> cond false p q)
+
+assume
+val cas (r:ref int) (u v:int) (#i:erased int)
+  : stt_atomic bool emp_inames 
+    (pts_to r i)
+    (fun b ->
+      cond b (pts_to r v ** pure (reveal i == u)) 
+             (pts_to r i))
+
+let trigger (x:'a) = emp
+
+```pulse
+fn atomic_increment_f5
+        (x: ref int)
+        (#invp #tok : vprop)
+        (#pred #qpred: int -> vprop)
+        (l:inv invp)
+        (elim_inv: 
+          (_:unit -> stt_ghost unit emp_inames invp (fun _ ->
+                    ((exists* v. pts_to x v ** pred v) ** tok))))
+        (intro_inv:
+            (_:unit -> stt_ghost unit emp_inames 
+                        ((exists* v. pts_to x v ** pred v) ** tok)
+                         (fun _ -> invp)))
+        (f: (v:int -> vq:int -> stt_ghost unit emp_inames 
+                  (pred v ** qpred vq ** pts_to x (v + 1))
+                  (fun _ -> pred (v + 1) ** qpred (vq + 1) ** pts_to x (v + 1))))
+requires qpred 'i
+ensures qpred ('i + 1)
+{
+  fn read ()
+  requires emp
+  returns v:int
+  ensures emp
+  {
+    0
+    //This doesn't work at the return type, complaining that it should be non-informative
+    // with_invariants l {
+        // elim_inv ();
+        // with i. _;
+        // share x;
+        // let v = atomic_read x;
+        // gather x;
+        // with _p. rewrite (pts_to x #_p v) as (pts_to x i);
+        // intro_inv ();
+        // v
+    // }
+  };
+  let mut continue = true;
+  fold (cond true (qpred 'i) (qpred ('i + 1)));
+  while (
+    with _b. _;
+    let b = !continue;
+    rewrite each _b as b;
+    b
+  )
+  invariant b.
+    pts_to continue b **
+    cond b (qpred 'i) (qpred ('i + 1))
+  {
+    let v = read ();
+    with_invariants l {
+        elim_inv ();
+        let b = cas x v (v + 1);
+        if b
+        {
+          elim_cond_true b _ _;
+          elim_cond_true true _ _;
+          f _ _;
+          // continue := false; //local variable assignment is considered non-atomic
+          intro_cond_false (qpred 'i) (qpred ('i + 1));
+          intro_inv ();
+          // show_proof_state; //the proof is done here, except for the assignment to continue
+          admit()
+        }
+        else
+        {
+          with p q. rewrite (cond b p q) as q;
+          intro_inv ();
+        }
+    }
+  };
+  with p q. unfold (cond false p q);
+}
+ 
+```
+
+
+assume
+val token : Type0
+
+assume
+val cancellable (t:token) (v:vprop) : vprop
+
+assume
+val active
+     (p:perm) 
+     (c:token)
+ : vprop
+
+assume
+val take (#p #t:_) (v:vprop) :
+  stt_ghost unit emp_inames
+    (cancellable t v ** active p t)
+    (fun _ -> v ** active p t)
+
+assume
+val restore (#p #t:_) (v:vprop) :
+  stt_ghost unit emp_inames
+    (v ** active p t)
+    (fun _ -> cancellable t v ** active p t)
+    
+
+assume
+val cancel (#t:_) (v:vprop) :
+  stt_ghost unit emp_inames
+    (cancellable t v ** active full_perm t)
+    (fun _ -> cancellable t v ** v)
+
+assume
+val create (v:vprop) :
+  stt_ghost (erased token) emp_inames v 
+          (fun t -> cancellable t v ** active full_perm t)
+
+assume
+val share (#p:_) (t:_) :
+  stt_ghost unit emp_inames
+    (active p t)
+    (fun _ -> active (half_perm p) t ** active (half_perm p) t)
+
+assume
+val gather (#p:_) (t:_) :
+  stt_ghost unit emp_inames
+    (active (half_perm p) t ** active (half_perm p) t)
+    (fun _ -> active p t)
+ 
+ assume
+ val cancel_inv (#t #v:_) (i:inv (cancellable t v)) :
+  stt_ghost unit emp_inames
+    (active full_perm t)
+    (fun _ -> v)
+
+
+```pulse
+fn atomic_increment_f6
+        (x: ref int)
+        (#p:_) (#t:erased token)
+        (#pred #qpred: int -> vprop)
+        (l:inv (cancellable t (exists* v. pts_to x v ** pred v)))
+        (f: (v:int -> vq:int -> stt_ghost unit emp_inames 
+                  (pred v ** qpred vq ** pts_to x (v + 1))
+                  (fun _ -> pred (v + 1) ** qpred (vq + 1) ** pts_to x (v + 1))))
+requires qpred 'i ** active p t
+ensures qpred ('i + 1) ** active p t
+{
+  with_invariants l {
+    take _;
+    atomic_increment x;
+    f _ 'i;
+    restore (exists* v. pts_to x v ** pred v)
+  }
+}
+```
+
+
+```pulse
+fn parallel_increment_inv
+        (x: ref int)
+requires pts_to x 'i
+ensures pts_to x ('i + 2)
+{
+    let left = GR.alloc #int 0;
+    let right = GR.alloc #int 0;
+    GR.share left;
+    GR.share right;
+    let tok = create (
+      exists* (v:int).
+          pts_to x v **
+          (exists* (vl vr:int).
+            GR.pts_to left #(half_perm full_perm) vl **
+            GR.pts_to right #(half_perm full_perm) vr **
+            pure (v == 'i + vl + vr))
+
+    );
+    share tok; 
+    let inv = new_invariant' (cancellable tok _);
+    ghost
+    fn step
+        (lr:GR.ref int)
+        (b:bool { if b then lr == left else lr == right })
+        (v vq:int)
+      requires 
+        (exists* (vl vr:int).
+            GR.pts_to left #(half_perm full_perm) vl **
+            GR.pts_to right #(half_perm full_perm) vr **
+            pure (v == 'i + vl + vr)) **
+        GR.pts_to lr #(half_perm full_perm) vq **
+        pts_to x (v + 1)
+      ensures
+        (exists* (vl vr:int).
+            GR.pts_to left #(half_perm full_perm) vl **
+            GR.pts_to right #(half_perm full_perm) vr **
+            pure (v + 1 == 'i + vl + vr)) **
+        GR.pts_to lr #(half_perm full_perm) (vq + 1) **
+        pts_to x (v + 1)
+    { 
+      if b
+      {
+        with _p _v. rewrite (GR.pts_to lr #_p _v) as (GR.pts_to left #_p _v);
+        GR.gather left;
+        with _p _v. rewrite (GR.pts_to left #_p _v) as (GR.pts_to left _v);
+        GR.( left := vq + 1 );
+        GR.share left;      
+        with _p _v. rewrite (GR.pts_to left #_p _v) as (GR.pts_to lr #_p _v);
+      }
+      else
+      {
+        with _p _v. rewrite (GR.pts_to lr #_p _v) as (GR.pts_to right #_p _v);
+        GR.gather right;
+        with _p _v. rewrite (GR.pts_to right #_p _v) as (GR.pts_to right _v);
+        GR.( right := vq + 1 );
+        GR.share right;      
+        with _p _v. rewrite (GR.pts_to right #_p _v) as (GR.pts_to lr #_p _v);
+      }
+    };
+
+    parallel
+    requires GR.pts_to left #(half_perm full_perm) 0 **
+             active (half_perm full_perm) tok
+         and GR.pts_to right #(half_perm full_perm) 0 **
+             active (half_perm full_perm) tok
+    ensures  GR.pts_to left #(half_perm full_perm) 1 **
+             active (half_perm full_perm) tok
+         and GR.pts_to right #(half_perm full_perm) 1 **
+             active (half_perm full_perm) tok
+    { atomic_increment_f6 x inv (step left true) }
+    { atomic_increment_f6 x inv (step right false) };
+
+    gather tok;
+    cancel_inv inv;
+    GR.gather left;
+    GR.gather right;
+    with _p _v. rewrite (GR.pts_to left #_p _v) as (GR.pts_to left _v);
+    with _p _v. rewrite (GR.pts_to right #_p _v) as (GR.pts_to right _v);
+    GR.free left;
+    GR.free right;
+
+}
+```
